Syntax and printing for decomposing declerations.

cpp2v-tests/test_decltype.cpp
@@ -8,6 +8,8 @@ int test() {
     int x = 0;
     decltype(x) y = 3;
     decltype((x)) z = x;
+#if __cplusplus < 201700
     typeof(x) p = 9;
+#endif
     return x;
 }
